src/BadSectorDisk/BadSectorImpl.v
@@ -1,0 +1,29 @@
+Require Import POCS.
+Require Import BadSectorAPI.
+
+
+Extraction Language Haskell.
+
+Module BadSectorDisk <: BadSectorAPI.
+
+  Axiom init : prog InitResult.
+  Axiom read : addr -> prog block.
+  Axiom write : addr -> block -> prog unit.
+  Axiom getBadSector : prog addr.
+  Axiom diskSize : prog nat.
+  Axiom recover : prog unit.
+
+  Axiom abstr : Abstraction State.
+
+  Axiom read_ok : forall a, prog_spec (read_spec a) (read a) recover abstr.
+  Axiom write_ok : forall a v, prog_spec (write_spec a v) (write a v) recover abstr.
+  Axiom getBadSector_ok : prog_spec getBadSector_spec getBadSector recover abstr.
+  Axiom diskSize_ok : prog_spec diskSize_spec diskSize recover abstr.
+  Axiom recover_noop : rec_noop recover abstr wipe.
+
+End BadSectorDisk.
+
+Extract Constant BadSectorDisk.read => "BadSectorDisk.Ops.read".
+Extract Constant BadSectorDisk.write => "BadSectorDisk.Ops.write".
+Extract Constant BadSectorDisk.getBadSector => "BadSectorDisk.Ops.getBadSector".
+Extract Constant BadSectorDisk.diskSize => "BadSectorDisk.Ops.diskSize".
